Move more stuff from fst to fsti.

src/Regs.fst
@@ -7,17 +7,3 @@ let n_reg_t : n:nat{0 < n} = 2
 let n_regtype _ : n:nat{0 < n} = 16
 
 let regval _ = nat
-
-let equal1 #_ f1 f2 = feq f1 f2
-
-let equal f1 f2 = forall t. equal1 (f1 t) (f2 t)
-
-let lemma_equal1_intro t regs1 regs2 = ()
-
-let lemma_equal1_elim t regs1 regs2 = ()
-
-let lemma_equal_intro regs1 regs2 = ()
-
-let lemma_equal_elim regs1 regs2 =
-	assert (equal regs1 regs2 ==> (forall t. regs1 t == regs2 t));
-	admit() (* help needed *)
